modq code

code/experimental/ed25519/Hacl.Impl.BignumQ.Mul.fst
@@ -1,4 +1,209 @@
 module Hacl.Impl.BignumQ.Mul
 
+open FStar.HyperStack
 open FStar.Buffer
+open Hacl.Cast
+open Hacl.UInt64
+
+open Hacl.Spec.BignumQ.Eval
+
+module Spec = Hacl.Spec.BignumQ.Mul
+
+#reset-options "--max_fuel 0 --max_ifuel 0 --z3rlimit 20"
+
+let h64 = Hacl.UInt64.t
+let qelemB = b:buffer h64{length b = 5}
+
+let within_56 (h:mem) (b:qelemB) : GTot Type0 =
+  live h b /\ (let b = as_seq h b in
+    v b.[0] < 0x100000000000000 /\ v b.[1] < 0x100000000000000 /\ v b.[2] < 0x100000000000000 /\ 
+    v b.[3] < 0x100000000000000 /\ v b.[4] < 0x100000000000000)
+
+val make_m:
+  m:qelemB ->
+  Stack unit
+    (requires (fun h -> live h m))
+    (ensures (fun h0 _ h1 -> live h1 m /\ modifies_1 m h0 h1
+      /\ as_seq h1 m == Spec.m))
+let make_m m =
+  Hacl.Lib.Create64.make_h64_5 m 0x12631a5cf5d3eduL 0xf9dea2f79cd658uL 0x000000000014deuL
+                              0x00000000000000uL 0x00000010000000uL
+
+val make_mu:
+  m:qelemB ->
+  Stack unit
+    (requires (fun h -> live h m))
+    (ensures (fun h0 _ h1 -> live h1 m /\ modifies_1 m h0 h1
+      /\ as_seq h1 m == Spec.mu))
+let make_mu m =
+  Hacl.Lib.Create64.make_h64_5 m 0x9ce5a30a2c131buL 0x215d086329a7eduL 0xffffffffeb2106uL
+                              0xffffffffffffffuL 0x00000fffffffffuL
+
+val choose:
+  z:qelemB ->
+  x:qelemB ->
+  y:qelemB ->
+  b:h64{v b == 0 \/ v b == 1} ->
+  Stack unit
+    (requires (fun h -> live h x /\ live h y /\ live h z))
+    (ensures (fun h0 _ h1 -> live h0 x /\ live h0 y /\ live h1 z /\ modifies_1 z h0 h1
+      /\ (as_seq h1 z == Spec.choose (as_seq h0 x) (as_seq h0 y) (b))))
+let choose z x y b =
+  let mask = b -%^ 1uL in
+  let x0 = x.(0ul) in
+  let x1 = x.(1ul) in
+  let x2 = x.(2ul) in
+  let x3 = x.(3ul) in
+  let x4 = x.(4ul) in
+  let y0 = y.(0ul) in
+  let y1 = y.(1ul) in
+  let y2 = y.(2ul) in
+  let y3 = y.(3ul) in
+  let y4 = y.(4ul) in
+  let z0 = ((y0 ^^ x0) &^ mask) ^^ x0 in
+  let z1 = ((y1 ^^ x1) &^ mask) ^^ x1 in
+  let z2 = ((y2 ^^ x2) &^ mask) ^^ x2 in
+  let z3 = ((y3 ^^ x3) &^ mask) ^^ x3 in
+  let z4 = ((y4 ^^ x4) &^ mask) ^^ x4 in
+  Hacl.Lib.Create64.make_h64_5 z z0 z1 z2 z3 z4
+
+
+let lt (a:h64{v a < pow2 63}) (b:h64{v b < pow2 63}) :
+  Tot (c:h64{if v a >= v b then v c == 0x0 else v c == 0x1})
+  = let r = (a -%^ b) >>^ 63ul in r
+
+let shiftl_56 (b:h64{b == 0uL \/ b == 1uL}) :
+  Tot (c:h64{(v b == 1 ==> v c == 0x100000000000000) /\ (v b == 0 ==> v c == 0)})
+  = assert_norm(pow2 56 = 0x100000000000000);
+    b <<^ 56ul
+
+open FStar.Mul
+
+inline_for_extraction
+val subm_step:
+  x:h64{v x < 0x100000000000000} ->
+  y:h64{v y <= 0x100000000000000} ->
+  Tot (t:(tuple2 h64 h64){
+    let b, t = t in
+    (v b == 0 \/ v b == 1)
+    /\ v x - v y == v t - 0x100000000000000 * v b
+    /\ v t < 0x100000000000000})
+let subm_step x y =
+  let b  = lt x y in
+  let t = (shiftl_56 b +^ x) -^ y in
+  b, t
+
+inline_for_extraction
+let shiftl_40 (b:u64{b == 0uL \/ b == 1uL}) :
+  Tot (c:u64{(b == 1uL ==> c == 0x10000000000uL) /\ (b == 0uL ==> c == 0uL)})
+  = assert_norm(pow2 40 = 0x10000000000);
+    b <<^ 40ul
+
+inline_for_extraction
+val subm_last_step:
+  x:u64{v x < 0x10000000000} ->
+  y:u64{v y <= 0x10000000000} ->
+  Tot (t:(tuple2 u64 u64){(fst t == 0uL \/ fst t == 1uL)
+    /\ v x - v y == v (snd t) - 0x10000000000 * v (fst t)
+    /\ v (snd t) < 0x10000000000})
+let subm_last_step x y =
+  let b  = lt x y in
+  let t = (shiftl_40 b +^ x) -^ y in
+  b, t
+
+#reset-options "--max_fuel 0 --max_ifuel 0 --z3rlimit 100"
+
+val sub_mod_264:
+  z:qelemB ->
+  x:qelemB ->
+  y:qelemB ->
+  Stack unit
+    (requires (fun h -> live h x /\ live h y /\ live h z
+      /\ within_56 h x /\ within_56 h y
+      /\ eval_q (as_seq h x) < pow2 264
+      /\ eval_q (as_seq h y) < pow2 264))
+    (ensures (fun h0 _ h1 -> live h0 x /\ live h0 y /\ live h1 z /\ modifies_1 z h0 h1
+      /\ within_56 h0 x /\ within_56 h0 y
+      /\ eval_q (as_seq h0 x) < pow2 264
+      /\ eval_q (as_seq h0 y) < pow2 264
+      /\ (as_seq h1 z == Spec.sub_mod_264 (as_seq h0 x) (as_seq h0 y))))
+let sub_mod_264 z x y =
+  assert_norm(pow2 264 = 0x1000000000000000000000000000000000000000000000000000000000000000000);
+  assert_norm(pow2 64 = 0x10000000000000000);
+  assert_norm(pow2 56 = 0x100000000000000);
+  assert_norm(pow2 40 = 0x10000000000);
+  assert_norm(pow2 32 = 0x100000000);
+  let x0 = x.(0ul) in
+  let x1 = x.(1ul) in
+  let x2 = x.(2ul) in
+  let x3 = x.(3ul) in
+  let x4 = x.(4ul) in
+  let y0 = y.(0ul) in
+  let y1 = y.(1ul) in
+  let y2 = y.(2ul) in
+  let y3 = y.(3ul) in
+  let y4 = y.(4ul) in
+  let pb = y0 in
+  (* let (b, t0) : Tot _ (\* : Tot (tuple2 h64 h64) *\) = subm_step x0 y0 <: Tot (tuple2 h64 h64) in *)
+  (* let (b, t1) (\* : Tot _) *\) = subm_step x1 (y1+^b) <: Tot (tuple2 h64 h64) in *)
+  (* let (b, t2) (\* : Tot _) *\) = subm_step x2 (y2+^b) <: Tot (tuple2 h64 h64) in *)
+  (* let (b, t3) (\* : Tot _)  *\)= subm_step x3 (y3+^b) <: Tot (tuple2 h64 h64) in *)
+  (* let (b, t4) (\* : Tot _) *\) = subm_last_step x4 (y4+^b) <: Tot (tuple2 h64 h64) in *)
+  let b  = lt x0 y0 in
+  let t0 = (shiftl_56 b +^ x0) -^ (y0) in
+  let y1 = y1 +^ b in
+  let b  = lt x1 (y1) in
+  let t1 = (shiftl_56 b +^ x1) -^ (y1) in
+  let y2 = y2 +^ b in
+  let b  = lt x2 (y2) in
+  let t2 = (shiftl_56 b +^ x2) -^ (y2) in
+  let y3 = y3 +^ b in
+  let b  = lt x3 (y3) in
+  let t3 = (shiftl_56 b +^ x3) -^ (y3) in
+  let y4 = y4 +^ b in
+  let b  = lt x4 (y4) in
+  let t4 = (shiftl_40 b +^ x4) -^ (y4) in
+  Hacl.Lib.Create64.make_h64_5 z t0 t1 t2 t3 t4
+
+val subm_conditional:
+  z:qelemB ->
+  x:qelemB ->
+  Stack unit
+    (requires (fun h -> live h x /\ live h z /\ within_56 h x))
+    (ensures (fun h0 _ h1 -> live h0 x /\ live h1 z /\ modifies_1 z h0 h1 /\ within_56 h0 x
+      /\ (as_seq h1 z == Spec.subm_conditional (as_seq h0 x))))
+let subm_conditional z x =
+  assert_norm(pow2 64 = 0x10000000000000000);
+  assert_norm(pow2 56 = 0x100000000000000);
+  assert_norm(pow2 32 = 0x100000000);
+  push_frame();
+  let tmp = create 0uL 5ul in
+  let x0 = x.(0ul) in
+  let x1 = x.(1ul) in
+  let x2 = x.(2ul) in
+  let x3 = x.(3ul) in
+  let x4 = x.(4ul) in
+  Hacl.Lib.Create64.make_h64_5 tmp x0 x1 x2 x3 x4;
+  let y0 = 0x12631a5cf5d3eduL in
+  let y1 = 0xf9dea2f79cd658uL in
+  let y2 = 0x000000000014deuL in
+  let y3 = 0x00000000000000uL in
+  let y4 = 0x00000010000000uL in
+  let b  = lt x0 y0 in
+  let t0 = (shiftl_56 b +^ x0) -^ (y0) in
+  let y1 = y1 +^ b in
+  let b  = lt x1 (y1) in
+  let t1 = (shiftl_56 b +^ x1) -^ (y1) in
+  let y2 = y2 +^ b in
+  let b  = lt x2 (y2) in
+  let t2 = (shiftl_56 b +^ x2) -^ (y2) in
+  let y3 = y3 +^ b in
+  let b  = lt x3 (y3) in
+  let t3 = (shiftl_56 b +^ x3) -^ (y3) in
+  let y4 = y4 +^ b in
+  let b  = lt x4 (y4) in
+  let t4 = (shiftl_56 b +^ x4) -^ (y4) in
+  Hacl.Lib.Create64.make_h64_5 z t0 t1 t2 t3 t4;
+  choose z tmp z b;
+  pop_frame()
 
